src/program_proof/pav/history.v
@@ -26,30 +26,39 @@ Definition msv_final (adtr_γ : gname) (ep uid : w64) (lat : lat_val_ty) : iProp
     "#His_label" ∷ is_vrf uid (W64 $ length vals) label ∗
     "%Hnin_map" ∷ ⌜ m !! label = None ⌝).
 
-Definition know_hist_val_cliG cli_γ (uid ep : w64) (hist : list map_val_ty) : iProp Σ :=
-  let vals := filter (λ x, uint.Z x.1 ≤ uint.Z ep) hist in
+(* TODO: add inv that says every key in cli submap will have a vrf. *)
+Definition know_hist_val_cliG cli_γ (uid ep : w64) (hist : list map_val_ty) (valid : w64) : iProp Σ :=
+  ∃ (vals : list opaque_map_val_ty),
+  "#Hpk_comm_reln" ∷
+    ([∗ list] pk_val;comm_val ∈ filter (λ x, uint.Z x.1 ≤ uint.Z ep) hist;vals,
+    "%Heq_ep" ∷ ⌜ pk_val.1 = comm_val.1⌝ ∗
+    "#Hcomm" ∷ is_comm pk_val.2 comm_val.2) ∗
   (* prior vers exist in prior or this map. *)
-  "#Hhist" ∷ ([∗ list] ver ↦ '(prior, pk) ∈ vals,
-    (∃ dig m_γ comm,
-    "%Hlt_prior" ∷ ⌜ uint.Z prior ≤ uint.Z ep ⌝ ∗
+  "#Hhist" ∷
+    ([∗ list] ver ↦ '(prior, comm) ∈ vals,
+    ∃ dig m_γ label,
     "#Hsubmap" ∷ mono_list_idx_own cli_γ (uint.nat prior) (Some (dig, m_γ)) ∗
-    "#Hcomm" ∷ is_comm pk comm ∗
-    "#Hin_prior" ∷ (uid, W64 ver) ↪[m_γ]□ Some (prior, comm))) ∗
-  ( (* next ver doesn't exist in this or later map. *)
-    "Hnin_nextver" ∷ (∃ (bound : w64) dig m_γ,
-      "%Hgte_bound" ∷ ⌜ uint.Z ep ≤ uint.Z bound ⌝ ∗
-      "#Hsubmap" ∷ mono_list_idx_own cli_γ (uint.nat bound) (Some (dig, m_γ)) ∗
-      "#Hin_bound" ∷ (uid, W64 $ length vals) ↪[m_γ]□ None)
+    "#Hin_prior" ∷ (uid, W64 ver) ↪[m_γ]□ Some (prior, comm) ∗
+    "#His_label" ∷ is_vrf uid (W64 ver) label) ∗
+  "#Hbound" ∷
+    (∃ (bound : w64) dig m_γ label,
+    "#Hsubmap" ∷ mono_list_idx_own cli_γ (uint.nat bound) (Some (dig, m_γ)) ∗
+    "#His_label" ∷ is_vrf uid (W64 $ length vals) label ∗
+    "%Hlt_bound" ∷ ⌜ uint.Z bound ≤ uint.Z valid ⌝ ∗
+    (* next ver doesn't exist in this or later map. *)
+    (("%Hgt_bound" ∷ ⌜ uint.Z ep ≤ uint.Z bound ⌝ ∗
+    "#Hin_bound" ∷ (uid, W64 $ length vals) ↪[m_γ]□ None)
     ∨
     (* next ver exists in later map. *)
-    "Hin_nextver" ∷ (∃ (bound : w64) dig m_γ comm,
-      "%Hgt_bound" ∷ ⌜ uint.Z ep < uint.Z bound ⌝ ∗
-      "#Hsubmap" ∷ mono_list_idx_own cli_γ (uint.nat bound) (Some (dig, m_γ)) ∗
-      "#Hin_bound" ∷ (uid, W64 $ length vals) ↪[m_γ]□ Some (bound, comm))).
+    (∃ comm,
+    "%Hgt_bound" ∷ ⌜ uint.Z ep < uint.Z bound ⌝ ∗
+    "#Hin_bound" ∷ (uid, W64 $ length vals) ↪[m_γ]□ Some (bound, comm)))).
 
-Definition know_hist_cliG cli_γ (uid : w64) (hist : list map_val_ty) (bound : w64) : iProp Σ :=
-  "%Hok_bound" ∷ ⌜ ∀ ep val, hist !! ep = Some val → uint.Z val.1 ≤ uint.Z bound ⌝ ∗
-  "#Hknow_vals" ∷ ∀ (ep : w64), ⌜ uint.Z ep ≤ uint.Z bound ⌝ -∗ know_hist_val_cliG cli_γ uid ep hist.
+Definition know_hist_cliG cli_γ (uid : w64) (hist : list map_val_ty) (valid : w64) : iProp Σ :=
+  "%Hok_valid" ∷ ⌜ ∀ i ep pk, hist !! i = Some (ep, pk) →
+    uint.Z ep ≤ uint.Z valid ⌝ ∗
+  "#Hknow_vals" ∷ (∀ (ep : w64), ⌜ uint.Z ep ≤ uint.Z valid ⌝ -∗
+    know_hist_val_cliG cli_γ uid ep hist valid).
 
 Definition own_HistEntry (ptr : loc) (obj : map_val_ty) : iProp Σ :=
   ∃ sl_HistVal,
@@ -57,11 +66,11 @@ Definition own_HistEntry (ptr : loc) (obj : map_val_ty) : iProp Σ :=
   "Hptr_HistVal" ∷ ptr ↦[HistEntry :: "HistVal"] (slice_val sl_HistVal) ∗
   "#Hsl_HistVal" ∷ own_slice_small sl_HistVal byteT DfracDiscarded obj.2.
 
-Definition own_hist cli_γ uid sl_hist hist bound : iProp Σ :=
+Definition own_hist cli_γ uid sl_hist hist valid : iProp Σ :=
   ∃ dim0_hist,
   "Hsl_hist" ∷ own_slice sl_hist ptrT (DfracOwn 1) dim0_hist ∗
   "Hdim0_hist" ∷ ([∗ list] p;o ∈ dim0_hist;hist, own_HistEntry p o) ∗
-  "#Hknow_hist" ∷ know_hist_cliG cli_γ uid hist bound.
+  "#Hknow_hist" ∷ know_hist_cliG cli_γ uid hist valid.
 End defs.
 
 Section derived.
@@ -93,47 +102,100 @@ Proof.
   rewrite filter_cons_True; [|done]. by rewrite IH.
 Qed.
 
-Lemma hist_extend_selfmon cli_γ uid hist bound new_bound :
-  uint.Z bound ≤ uint.Z new_bound →
-  ("#Hknow_hist" ∷ know_hist_cliG cli_γ uid hist bound ∗
-  "#His_bound" ∷ is_my_bound cli_γ uid (W64 $ length hist) new_bound) -∗
-  "#Hknow_hist" ∷ know_hist_cliG cli_γ uid hist new_bound.
+Lemma hist_val_extend_valid γ uid ep hist valid new_valid :
+  uint.Z valid ≤ uint.Z new_valid →
+  know_hist_val_cliG γ uid ep hist valid -∗
+  know_hist_val_cliG γ uid ep hist new_valid.
+Proof.
+  intros ?. iNamed 1. iNamed "Hbound". iExists vals. iFrame "#".
+  iDestruct "Hbound" as "[Hbound|Hbound]"; iNamed "Hbound"; iPureIntro; word.
+Qed.
+
+Lemma hist_extend_selfmon cli_γ uid hist valid new_valid :
+  uint.Z valid ≤ uint.Z new_valid →
+  ("#Hknow_hist" ∷ know_hist_cliG cli_γ uid hist valid ∗
+  "#His_bound" ∷ is_my_bound cli_γ uid (W64 $ length hist) new_valid) -∗
+  "#Hknow_hist" ∷ know_hist_cliG cli_γ uid hist new_valid.
 Proof.
   intros ?. iNamed 1. iNamed "Hknow_hist". iSplit.
-  { iIntros (?? Hlook). iPureIntro. specialize (Hok_bound _ _ Hlook). word. }
-  iIntros (ep ?). destruct (decide (uint.Z ep ≤ uint.Z bound)).
-  { by iApply "Hknow_vals". }
-  iSpecialize ("Hknow_vals" $! bound with "[]"). { iPureIntro. lia. }
-  iSplit.
-  - iNamed "Hknow_vals".
-    rewrite (list_filter_iff_strong
+  { iIntros (??? Hlook) "!%". specialize (Hok_valid _ _ _ Hlook). word. }
+  iIntros (ep ?). destruct (decide (uint.Z ep ≤ uint.Z valid)).
+  { iSpecialize ("Hknow_vals" $! ep with "[]"). { iPureIntro. word. }
+    iApply (hist_val_extend_valid with "Hknow_vals"). word. }
+  iSpecialize ("Hknow_vals" $! valid with "[]"). { iPureIntro. lia. }
+  iNamed "Hknow_vals". iExists vals. iSplit; [|iSplit].
+  - rewrite (list_filter_iff_strong
       (λ x, uint.Z x.1 ≤ uint.Z ep)
-      (λ x, uint.Z x.1 ≤ uint.Z bound) hist); [|naive_solver word].
-    iApply (big_sepL_impl with "Hhist"). iIntros (?[??]) "!> %". iNamed 1.
-    iFrame "#". iPureIntro. word.
-  - iClear "Hknow_vals". iLeft.
-    rewrite list_filter_all; last first.
-    { intros ?? Hlook. ospecialize (Hok_bound _ _ Hlook). word. }
-    iNamed "His_bound". iFrame "#". iPureIntro. word.
+      (λ x, uint.Z x.1 ≤ uint.Z valid) hist); last first.
+    { intros ?[??] Hlook. ospecialize (Hok_valid _ _ _ Hlook).
+      naive_solver word. }
+    iFrame "#".
+  - iFrame "#".
+  - iClear "Hhist Hbound".
+    iDestruct (big_sepL2_length with "Hpk_comm_reln") as %Hlen_vals.
+    rewrite list_filter_all in Hlen_vals; last first.
+    { intros ?[??] Hlook. ospecialize (Hok_valid _ _ _ Hlook). simpl. word. }
+    iNamed "His_bound". rewrite Hlen_vals. by iFrame "#%".
 Qed.
 
 Definition get_lat (hist : list map_val_ty) (ep : w64) : lat_val_ty :=
   last $ filter (λ x, uint.Z x.1 ≤ uint.Z ep) hist.
 
-Lemma hist_audit_msv cli_γ uid hist bound adtr_γ aud_ep (ep : w64) :
-  uint.Z ep ≤ uint.Z bound →
-  uint.Z bound < uint.Z aud_ep →
-  ("#Hknow_hist" ∷ know_hist_cliG cli_γ uid hist bound ∗
+Lemma hist_audit_msv cli_γ uid hist valid adtr_γ aud_ep (ep : w64) :
+  uint.Z ep ≤ uint.Z valid →
+  uint.Z valid < uint.Z aud_ep →
+  ("#Hknow_hist" ∷ know_hist_cliG cli_γ uid hist valid ∗
   "#His_audit" ∷ is_audit cli_γ adtr_γ aud_ep) -∗
   "#Hmsv" ∷ msv_final adtr_γ ep uid (get_lat hist ep).
 Proof.
   intros ??. iNamed 1.
-  rewrite /msv_final.
-  iNamed "Hknow_hist".
-  iSpecialize ("Hknow_vals" $! ep with "[//]"). iNamed "Hknow_vals".
-  iNamed "His_audit".
-  rewrite /is_audit.
-Admitted.
+  iNamed "Hknow_hist". iSpecialize ("Hknow_vals" $! ep with "[//]").
+  iDestruct "His_audit" as (ms) "His_audit". iNamed "His_audit".
+  list_elem ms (uint.nat ep) as m.
+  iDestruct (mono_list_idx_own_get _ _ Hm_lookup with "Hadtr_maps") as "Hadtr_map".
+  iFrame "Hadtr_map".
+  iDestruct "Hknow_vals" as (vals) "Hknow_vals". iExists vals.
+  iNamed "Hknow_vals". iSplit; [|iSplit].
+  - iClear "Hhist Hbound".
+    iDestruct (big_sepL2_length with "Hpk_comm_reln") as %Hlen_vals.
+    destruct (get_lat hist ep) as [[??]|] eqn:Hlat_pk, (last vals) as [[??]|] eqn:Hlat_comm;
+      [|exfalso..|done];
+      rewrite /get_lat last_lookup in Hlat_pk; rewrite last_lookup in Hlat_comm.
+    + rewrite Hlen_vals in Hlat_pk.
+      iDestruct (big_sepL2_lookup with "Hpk_comm_reln") as "?"; [exact Hlat_pk|exact Hlat_comm|].
+      iFrame "#".
+    + apply lookup_lt_Some in Hlat_pk. apply lookup_ge_None in Hlat_comm. lia.
+    + apply lookup_ge_None in Hlat_pk. apply lookup_lt_Some in Hlat_comm. lia.
+  - iClear "Hbound".
+    iApply (big_sepL_impl with "Hhist"). iIntros (?[prior ?]) "!> %Hlook_vals". iNamed 1. iFrame "#".
+    (* tedious: trace prior ep back to filtered hist to get filter bound on it. *)
+    iDestruct (big_sepL2_lookup_2_some with "Hpk_comm_reln") as %[[??] Hlook_hist]; [exact Hlook_vals|].
+    iDestruct (big_sepL2_lookup with "Hpk_comm_reln") as "Htmp"; [exact Hlook_hist|exact Hlook_vals|].
+    iNamed "Htmp". opose proof (proj1 (elem_of_list_filter _ _ _) _) as [? _].
+    { eapply elem_of_list_lookup. eauto using Hlook_hist. }
+    simpl in *. list_elem ms (uint.nat prior) as mprior.
+    iDestruct ("Hmap_transf" with "[$Hsubmap $Hin_prior $His_label]") as "Htmp".
+    { iPureIntro. exact Hmprior_lookup. }
+    iNamed "Htmp". iPureIntro.
+    opose proof ((proj1 Hinv_adtr) _ _ _ _ Hmprior_lookup Hm_lookup _); [word|].
+    by eapply lookup_weaken.
+  - iClear "Hhist". iNamed "Hbound". iFrame "#".
+    list_elem ms (uint.nat bound) as mbound.
+    iDestruct "Hbound" as "[Hbound|Hbound]"; iNamed "Hbound".
+    + iSpecialize ("Hmap_transf" with "[$Hsubmap $Hin_bound $His_label]").
+      { iPureIntro. exact Hmbound_lookup. }
+      iNamed "Hmap_transf". iPureIntro.
+      opose proof ((proj1 Hinv_adtr) _ _ _ _ Hm_lookup Hmbound_lookup _); [word|].
+      by eapply lookup_weaken_None.
+    + iSpecialize ("Hmap_transf" with "[$Hsubmap $Hin_bound $His_label]").
+      { iPureIntro. exact Hmbound_lookup. }
+      iNamed "Hmap_transf". iPureIntro.
+      destruct (decide $ is_Some $ m !! label) as [[? Hlook_mkey]|]; last first.
+      { by eapply eq_None_not_Some. }
+      opose proof ((proj1 Hinv_adtr) _ _ _ _ Hm_lookup Hmbound_lookup _); [word|].
+      opose proof (lookup_weaken _ _ _ _ Hlook_mkey _); [done|]. simplify_eq/=.
+      opose proof ((proj2 Hinv_adtr) _ _ _ _ _ Hm_lookup Hlook_mkey) as ?. word.
+Qed.
 
 End derived.
 
